varsAllocated for a PC continued

Clap/eDSLState/Circuit.lean
@@ -1,5 +1,6 @@
 import Mathlib.Control.Monad.Writer
 
+import Clap.BitVec
 import Clap.eDSLState.HashCons.CacheExpr
 import Clap.eDSLState.HashCons.EvalButActuallyGood
 import Clap.eDSLState.Varstore
@@ -7,46 +8,75 @@ import Clap.eDSLState.Varstore
 namespace Clap
 
 @[grind cases]
-inductive CircuitusPlanus (p : ℕ) where
+inductive Gate (p : ℕ) where
   | eq0 (e : ExprRef)
   | share (e : ExprRef)
   | isZero (e : ExprRef)
   | num2bits (w : ℕ) (e : ExprRef)
 
 @[grind =]
-def CircuitusPlanus.refsValid {p : ℕ} (c : CircuitusPlanus p) (bound : ℕ) : Prop := match c with
+def Gate.refsValid {p : ℕ} (c : Gate p) (bound : ℕ) : Prop := match c with
   | .eq0 e => e < bound
   | .share e => e < bound
   | .isZero e => e < bound
   | .num2bits _w e => e < bound
 
 @[grind =]
-def CircuitusPlanus.varsAllocated {p : ℕ} (c : CircuitusPlanus p) (varStore : VarStore p) (σ : HashConsSt p) : Prop := match c with
+def Gate.varsAllocated {p : ℕ} (c : Gate p) (varStore : VarStore p) (σ : HashConsSt p) : Prop := match c with
     | .eq0 e => [varStore, σ|e].isSome
     | .share e => [varStore, σ|e].isSome
     | .isZero e => [varStore, σ|e].isSome
     | .num2bits _w e => [varStore, σ|e].isSome
 
-instance {p : ℕ} {c : CircuitusPlanus p} {varStore : VarStore p} {σ : HashConsSt p} :
+instance {p : ℕ} {c : Gate p} {varStore : VarStore p} {σ : HashConsSt p} :
   Decidable (c.varsAllocated varStore σ) := by
-  unfold CircuitusPlanus.varsAllocated
+  unfold Gate.varsAllocated
   rcases c <;> infer_instance 
 
-instance {p: ℕ} {x : CircuitusPlanus p} {bound : ℕ}: Decidable (x.refsValid bound) := match x with
+instance {p: ℕ} {x : Gate p} {bound : ℕ}: Decidable (x.refsValid bound) := match x with
   | .eq0 e => e.decLt bound
   | .share e => e.decLt bound
   | .isZero e => e.decLt bound
   | .num2bits _w e => e.decLt bound
 
-abbrev CircuitState (p : ℕ) := Array (CircuitusPlanus p)
+abbrev Circuit (p : ℕ) := Array (Gate p)
 
 @[grind =]
-def CircuitState.refsValid {p : ℕ} (c : CircuitState p) (bound : ℕ) : Prop :=
+def Circuit.refsValid {p : ℕ} (c : Circuit p) (bound : ℕ) : Prop :=
   c.all λ x => (decide (x.refsValid bound))
 
 @[grind =]
-def CircuitState.varsAllocated {p : ℕ} (c : CircuitState p) (varStore : VarStore p) (σ : HashConsSt p) (pc : ℕ) : Prop :=
+def Circuit.varsAllocated {p : ℕ} (c : Circuit p) (varStore : VarStore p) (σ : HashConsSt p) (pc : ℕ) : Prop :=
   ∀ i < pc, c[pc]?.any fun instr ↦ instr.varsAllocated varStore σ
+
+structure State where
+  numAlloc : ℕ
+  pc : ℕ
+deriving Inhabited
+
+namespace State
+
+def addAlloc (st : State) (k : ℕ) : State :=
+  {st with numAlloc := st.numAlloc + k}
+
+def bumpAlloc (st : State) : State :=
+  st.addAlloc 1
+
+def addPc (st : State) (k : ℕ) : State :=
+  {st with pc := st.pc + k}
+
+def bumpPc (st : State) : State :=
+  st.addPc 1
+
+section Lemmas
+
+variable {st : State}
+
+lemma bumpPc_eq : st.bumpPc = {st with pc := st.pc + 1} := rfl
+
+end Lemmas
+
+end State
 
 -- isZero : input → Bool
 -- need to allocate the output of this thing
@@ -61,7 +91,7 @@ def CircuitState.varsAllocated {p : ℕ} (c : CircuitState p) (varStore : VarSto
 namespace Edsl
 
 structure CircuitResult (p : ℕ) where
-  numAlloc : ℕ
+  st : State
   varStore : VarStore p
   constraints : Prop
   deriving Inhabited
@@ -71,49 +101,53 @@ namespace CircuitResult
 section
 
 -- TODO do we need all of these?
-variable {p k numAlloc : ℕ} {result result' : CircuitResult p}
-         {constraint : Prop} {vars : Vector (ZMod p) k} {e : HashConsM p ExprRef} {e! : ExprRef}
+variable {p k numAlloc : ℕ} {result result' : CircuitResult p} {st : State}
+         {constraint constraints : Prop} {vars : Vector (ZMod p) k} {e : HashConsM p ExprRef} {e! : ExprRef}
          {varStore : VarStore p}
-         {σ : HashConsSt p}
+         {σ : HashConsSt p} {vars : Vector (ZMod p) k}
 
-def init (p : ℕ) : CircuitResult p := ⟨0, ∅, True⟩
+def init (p : ℕ) : CircuitResult p := ⟨⟨0, 0⟩, ∅, True⟩
 
-def unconstrained (numAlloc : ℕ) (varStore : VarStore p) : CircuitResult p :=
-  ⟨numAlloc, varStore, True⟩
+def unconstrained (st : State) (varStore : VarStore p) : CircuitResult p :=
+  ⟨st, varStore, True⟩
+
+@[grind =]
+def bumpPc {p : ℕ} (result : CircuitResult p) : CircuitResult p :=
+  {result with st := result.st.bumpPc}
+
+variable {result : CircuitResult p}
 
 notation (name := notationα) "unconstrained[" numAlloc:arg "]" "[" varStore:arg "]" => unconstrained numAlloc varStore
 
 recommended_spelling "unconstrained" for "α" in [unconstrained, notationα]
 
 @[simp, grind =]
-lemma numAlloc_unconstrained : unconstrained[numAlloc][varStore].numAlloc = numAlloc := rfl
+lemma numAlloc_unconstrained : unconstrained[st][varStore].st = st := rfl
 
 @[simp, grind =]
-lemma varStore_unconstrained : unconstrained[numAlloc][varStore].varStore = varStore := rfl
+lemma varStore_unconstrained : unconstrained[st][varStore].varStore = varStore := rfl
 
 @[simp, grind =]
-lemma constraints_unconstrained : unconstrained[numAlloc][varStore].constraints = True := rfl
+lemma constraints_unconstrained : unconstrained[st][varStore].constraints = True := rfl
 
 def addConstraint (result : CircuitResult p) (constraint : Prop) : CircuitResult p :=
   {result with constraints := result.constraints ∧ constraint}
 
 @[simp, grind =]
 lemma addConstraint_mk
-  (numAlloc : ℕ)
-  (varStore : VarStore p)
-  (constraints constraint : Prop)
+  {constraints constraint : Prop}
 :
-  (Edsl.CircuitResult.mk numAlloc varStore constraints).addConstraint constraint =
-  Edsl.CircuitResult.mk numAlloc varStore (constraints ∧ constraint)
+  (Edsl.CircuitResult.mk st varStore constraints).addConstraint constraint =
+  Edsl.CircuitResult.mk st varStore (constraints ∧ constraint)
 := rfl
 
 @[simp, grind =]
 lemma addConstraint_unconstrained {constraint : Prop} :
-  unconstrained[numAlloc][varStore].addConstraint constraint =
-  ⟨numAlloc, varStore, constraint⟩ := by simp [unconstrained]
+  unconstrained[st][varStore].addConstraint constraint =
+  ⟨st, varStore, constraint⟩ := by simp [unconstrained]
 
 @[simp, grind =]
-lemma numAlloc_addConstraint : (result.addConstraint constraint).numAlloc = result.numAlloc := rfl
+lemma numAlloc_addConstraint : (result.addConstraint constraint).st = result.st := rfl
 
 @[simp, grind =]
 lemma varStore_addConstraint : (result.addConstraint constraint).varStore = result.varStore := rfl
@@ -123,25 +157,22 @@ lemma constraints_addConstraint : (result.addConstraint constraint).constraints 
                                   (result.constraints ∧ constraint) := rfl
 
 def allocAnonymous (result : CircuitResult p) : CircuitResult p :=
-  {result with numAlloc := result.numAlloc + 1}
+  {result with st := result.st.bumpAlloc}
 
 @[simp, grind =]
 lemma allocAnonymous_mk
-  {numAlloc : ℕ}
-  {varStore : VarStore p}
-  {constraints : Prop}
 :
-  (Edsl.CircuitResult.mk numAlloc varStore constraints).allocAnonymous =
-  Edsl.CircuitResult.mk (numAlloc + 1) varStore constraints
+  (Edsl.CircuitResult.mk st varStore constraints).allocAnonymous =
+  Edsl.CircuitResult.mk st.bumpAlloc varStore constraints
 := rfl
 
 @[simp, grind =]
 lemma allocAnonymous_unconstrained :
-  unconstrained[numAlloc][varStore].allocAnonymous =
-  ⟨numAlloc + 1, varStore, True⟩ := by rfl
+  unconstrained[st][varStore].allocAnonymous =
+  ⟨st.bumpAlloc, varStore, True⟩ := rfl
 
 @[simp, grind =]
-lemma numAlloc_allocAnonymous : result.allocAnonymous.numAlloc = result.numAlloc + 1 := rfl
+lemma numAlloc_allocAnonymous : result.allocAnonymous.st = result.st.bumpAlloc := rfl
 
 @[simp, grind =]
 lemma varStore_allocAnonymous : result.allocAnonymous.varStore = result.varStore := rfl
@@ -183,54 +214,40 @@ lemma getDM_eq_getM?_getD : result.getDM e = result.getM? e <&> Option.getD (dfl
 
 @[simp, grind =]
 lemma get?_mk
-  {varStore : VarStore p}
-  {e : ExprRef}
-  {numAlloc : ℕ}
-  {constraints : Prop}
 :
-  (Edsl.CircuitResult.mk numAlloc varStore constraints).get? e σ =
-  [varStore,σ|e]
+  (Edsl.CircuitResult.mk st varStore constraints).get? e! σ =
+  [varStore,σ|e!]
 := rfl
 
 @[simp, grind =]
 lemma getM?_mk
-  {varStore : VarStore p}
-  {e : HashConsM p ExprRef}
-  (numAlloc : ℕ)
-  (constraints : Prop)
 :
-  ((Edsl.CircuitResult.mk numAlloc varStore constraints).getM? e).run σ =
+  ((Edsl.CircuitResult.mk st varStore constraints).getM? e).run σ =
   [varStore,σ|←e]
 := rfl
 
 @[simp, grind =]
 lemma getElem?_mk
-  {varStore : VarStore p}
-  {e : ExprRef}
-  {numAlloc : ℕ}
-  {constraints : Prop}
 :
-  (Edsl.CircuitResult.mk numAlloc varStore constraints)[(e, σ)]? =
-  [varStore,σ|e]
+  (Edsl.CircuitResult.mk st varStore constraints)[(e!, σ)]? =
+  [varStore,σ|e!]
 := rfl
 
 @[simp, grind =]
 lemma membership_unconstrained
-  {e :ExprRef}
 :
-  ((e, σ) ∈ unconstrained[numAlloc][varStore]) = [varStore,σ|e].isSome
+  ((e!, σ) ∈ unconstrained[st][varStore]) = [varStore,σ|e!].isSome
 := rfl
 
 @[simp, grind =]
 lemma getElem?_unconstrained
-  {e : ExprRef}
 :
-  unconstrained[numAlloc][varStore][(e, σ)]? = [varStore,σ|e]
+  unconstrained[st][varStore][(e!, σ)]? = [varStore,σ|e!]
 := rfl
 
 @[simp, grind =]
 lemma getM?_unconstrained:
-  (unconstrained[numAlloc][varStore].getM? e).run σ =
+  (unconstrained[st][varStore].getM? e).run σ =
   [varStore,σ|←e] := by simp [unconstrained]
 
 @[grind =>]
@@ -256,29 +273,21 @@ def assertAllocatedM (result : CircuitResult p) (e : HashConsM p ExprRef) : Hash
 
 @[simp, grind =]
 lemma assertAllocated_mk
-  {e : ExprRef}
-  {numAlloc : ℕ}
-  {varStore : VarStore p}
-  {constraints : Prop}
 :
-  (Edsl.CircuitResult.mk numAlloc varStore constraints).assertAllocated e σ =
+  (Edsl.CircuitResult.mk st varStore constraints).assertAllocated e! σ =
   Edsl.CircuitResult.mk
-    numAlloc
+    st
     varStore
-    (constraints ∧ [varStore,σ|e].isSome)
+    (constraints ∧ [varStore,σ|e!].isSome)
 := rfl
 
 @[simp, grind =]
 lemma assertAllocatedM_mk
-  {e : HashConsM p ExprRef}
-  {numAlloc : ℕ}
-  {varStore : VarStore p}
-  {constraints : Prop}
 :
-  ((Edsl.CircuitResult.mk numAlloc varStore constraints).assertAllocatedM e).run σ =
+  ((Edsl.CircuitResult.mk st varStore constraints).assertAllocatedM e).run σ =
   (
     Edsl.CircuitResult.mk
-      numAlloc
+      st
       varStore
       (constraints ∧ [varStore,σ|←e].1.isSome)
     ,
@@ -288,7 +297,7 @@ lemma assertAllocatedM_mk
 
 @[simp, grind =]
 lemma numAlloc_assertAllocated :
-  (result.assertAllocated e! σ).numAlloc = result.numAlloc := rfl
+  (result.assertAllocated e! σ).st = result.st := rfl
 
 @[simp, grind =]
 lemma varStore_assertAllocated :
@@ -300,48 +309,47 @@ lemma constraints_assertAllocated :
 
 @[simp, grind =]
 lemma assertAllocated_unconstrained :
-  unconstrained[numAlloc][varStore].assertAllocated e! σ =
-  letI α := unconstrained[numAlloc][varStore]
+  unconstrained[st][varStore].assertAllocated e! σ =
+  letI α := unconstrained[st][varStore]
   α.addConstraint ((e!, σ) ∈ α) := rfl
 
 def alloc {k p : ℕ} (result : CircuitResult p) (vals : Vector (ZMod p) k) : CircuitResult p :=
-  let indexed := (Vector.range k).map (·+result.numAlloc) |>.zip vals
+  let indexed := (Vector.range k).map (·+result.st.numAlloc) |>.zip vals
   let varStore := result.varStore.insertMany indexed
-  {result with varStore := varStore, numAlloc := result.numAlloc + k}
+  {result with varStore := varStore, st := result.st.addAlloc k}
 
 @[simp, grind =]
 lemma alloc_mk
-  (vals : Vector (ZMod p) k)
-  (numAlloc : ℕ)
-  (varStore : VarStore p)
-  (constraints : Prop)
+  {vals : Vector (ZMod p) k}
 :
-  (Edsl.CircuitResult.mk numAlloc varStore constraints).alloc vals =
+  (Edsl.CircuitResult.mk st varStore constraints).alloc vals =
   Edsl.CircuitResult.mk
-    (numAlloc + k)
-    (varStore.insertMany ((Vector.range k).map (·+numAlloc) |>.zip vals))
+    (st.addAlloc k)
+    (varStore.insertMany ((Vector.range k).map (·+st.numAlloc) |>.zip vals))
     constraints
 := rfl
 
 @[simp, grind =]
-lemma numAlloc_alloc {vars : Vector (ZMod p) k} :
-  (result.alloc vars).numAlloc = result.numAlloc + k := rfl
+lemma numAlloc_alloc :
+  (result.alloc vars).st = result.st.addAlloc k := rfl
 
 @[simp, grind =]
-lemma varStore_alloc {vars : Vector (ZMod p) k} :
+lemma varStore_alloc :
   (result.alloc vars).varStore =
-  result.varStore.insertMany ((Vector.range k).map (·+result.numAlloc) |>.zip vars) := rfl
+  result.varStore.insertMany ((Vector.range k).map (·+result.st.numAlloc) |>.zip vars) := rfl
 
 @[simp, grind =]
 lemma constraints_alloc {vars : Vector (ZMod p) k} :
   (result.alloc vars).constraints = result.constraints := rfl
 
-def step (result : CircuitResult p) (next : CircuitusPlanus p) (σ : HashConsSt p) : CircuitResult p :=
-  match next with
-  | .eq0 e => result.addConstraint (result[(e, σ)]? = .some 0)
-  | .share e => (result.assertAllocated e σ).alloc #v[result[(e, σ)]!]
-  | .isZero e => (result.assertAllocated e σ).alloc #v[if result[(e, σ)]? = .some 0 then 1 else 0]
-  | .num2bits width e => (result.assertAllocated e σ).alloc (num2bitsLsbPureV width (result[(e, σ)]!))
+def step (result : CircuitResult p) (next : Gate p) (σ : HashConsSt p) : CircuitResult p :=
+  let result :=
+    match next with
+    | .eq0 e => result.addConstraint (result[(e, σ)]? = Option.some 0)
+    | .share e => (result.assertAllocated e σ).alloc #v[result[(e, σ)]!]
+    | .isZero e => (result.assertAllocated e σ).alloc #v[if result[(e, σ)]? = Option.some 0 then 1 else 0]
+    | .num2bits width e => (result.assertAllocated e σ).alloc (num2bitsLsbPureV width (result[(e, σ)]!))
+  result.bumpPc
 
 notation "[" res ", " σ "|" cmd "]ₛ" => step res cmd σ
 
@@ -351,7 +359,7 @@ notation "[" res ", " σ "|" cmd "]ₛ" => step res cmd σ
 --   (numAlloc : ℕ)
 --   (varStore : VarStore p)
 --   (constraints : Prop)
---   (next : CircuitusPlanus p)
+--   (next : Gate p)
 -- : (Edsl.CircuitResult.mk numAlloc varStore constraints).step next =
 --   Edsl.CircuitResult.mk
 --     (match next with
@@ -383,15 +391,15 @@ notation "[" res ", " σ "|" cmd "]ₛ" => step res cmd σ
 --   -- rfl
 
 -- @[simp, grind =]
-lemma step_unconstrained {command : CircuitusPlanus p} {σ} :
-  [unconstrained[numAlloc][varStore], σ|command]ₛ =
-  [⟨numAlloc, varStore, True⟩, σ|command]ₛ := rfl
+lemma step_unconstrained {command : Gate p} {σ} :
+  [unconstrained[st][varStore], σ|command]ₛ =
+  [⟨st, varStore, True⟩, σ|command]ₛ := rfl
 
 def split (result : CircuitResult p) : CircuitResult p :=
   {result with constraints := True}
 
 @[simp, grind =]
-lemma numAlloc_split : result.split.numAlloc = result.numAlloc := rfl
+lemma numAlloc_split : result.split.st = result.st := rfl
 
 @[simp, grind =]
 lemma varStore_split : result.split.varStore = result.varStore := rfl
@@ -405,38 +413,38 @@ lemma constraints_split : result.split.constraints = True := rfl
 
 @[simp, grind =]
 lemma step_eq0 :
-  [result,σ|.eq0 e!]ₛ = result.addConstraint (result[(e!, σ)]? = .some 0) := rfl
+  [result,σ|.eq0 e!]ₛ = (result.addConstraint (result[(e!, σ)]? = .some 0)).bumpPc := rfl
 
 @[simp, grind =]
 lemma step_share :
   [result, σ|.share e!]ₛ =
-  (result.assertAllocated e! σ |>.alloc #v[result.getD e! σ]) := rfl
+  (result.assertAllocated e! σ |>.alloc #v[result.getD e! σ]).bumpPc := rfl
 
 @[simp, grind =]
 lemma step_isZero :
   [result, σ|.isZero e!]ₛ =
-  (result.assertAllocated e! σ |>.alloc #v[if result[(e!, σ)]? = .some 0 then 1 else 0]) := rfl
+  (result.assertAllocated e! σ |>.alloc #v[if result[(e!, σ)]? = .some 0 then 1 else 0]).bumpPc := rfl
 
 @[simp, grind =]
 lemma step_num2bits {width} :
   [result, σ|.num2bits width e!]ₛ =
-  (result.assertAllocated e! σ |>.alloc (num2bitsLsbPureV width result[(e!, σ)]!)) := rfl
+  (result.assertAllocated e! σ |>.alloc (num2bitsLsbPureV width result[(e!, σ)]!)).bumpPc := rfl
 
 @[aesop unsafe, grind =]
 lemma addConstraint_eq_mk :
   result.addConstraint constraint =
-  ⟨result.numAlloc, result.varStore, result.constraints ∧ constraint⟩ := rfl
+  ⟨result.st, result.varStore, result.constraints ∧ constraint⟩ := rfl
 
 @[aesop unsafe, grind =]
 lemma allocAnonymous_eq_mk :
   result.allocAnonymous =
-  ⟨result.numAlloc + 1, result.varStore, result.constraints⟩ := rfl
+  ⟨result.st.bumpAlloc, result.varStore, result.constraints⟩ := rfl
 
 lemma alloc_eq_mk {k} {vals : Vector _ k} :
   result.alloc vals =
-  ⟨result.numAlloc + k,
-   result.varStore.insertMany (((Vector.range k).map (· + result.numAlloc)).zip vals),
-   result.constraints⟩ := by rfl
+  ⟨result.st.addAlloc k,
+   result.varStore.insertMany (((Vector.range k).map (· + result.st.numAlloc)).zip vals),
+   result.constraints⟩ := rfl
 
 lemma assertAllocated_eq_addConstraint :
   result.assertAllocated e! σ = result.addConstraint ((e!, σ) ∈ result) := rfl
@@ -445,38 +453,33 @@ end
 
 end CircuitResult
 
-abbrev CircuitState.evalInOrder {p : ℕ} (circuit : CircuitState p) (σ : HashConsSt p) :=
+abbrev Circuit.evalInOrder {p : ℕ} (circuit : Circuit p) (σ : HashConsSt p) :=
   circuit.foldl (CircuitResult.step (σ := σ))
 
-def CircuitState.eval {p : ℕ} (circuit : CircuitState p) (varStore : VarStore p) (numAlloc : ℕ) (σ : HashConsSt p) : CircuitResult p :=
-  CircuitState.evalInOrder circuit σ ⟨numAlloc, varStore, True⟩
+def Circuit.eval {p : ℕ} (circuit : Circuit p) (varStore : VarStore p) (st : State) (σ : HashConsSt p) : CircuitResult p :=
+  Circuit.evalInOrder circuit σ ⟨st, varStore, True⟩
 
-notation "[" varStore ", " σ ", " numAlloc "|" circuit "]ₑ" => CircuitState.eval circuit varStore numAlloc σ
+notation "[" varStore ", " σ ", " numAlloc "|" circuit "]ₑ" => Circuit.eval circuit varStore numAlloc σ
 
 namespace CircuitResult
 
-variable {p : ℕ} {σ : HashConsSt p}
+variable {p : ℕ} {σ : HashConsSt p} {constraints1 constraints2 : Prop} {st : State}
+         {varStore : VarStore p} {circuit : Circuit p} {e! : ExprRef}
 
 @[ext, grind ext]
 lemma ext {p : ℕ} {r1 r2 : CircuitResult p}
-  (h_numAlloc : r1.numAlloc = r2.numAlloc)
+  (h_numAlloc : r1.st = r2.st)
   (h_varStore : r1.varStore = r2.varStore)
   (h_constraints : r1.constraints = r2.constraints)
 :
   r1 = r2
 := by
-  obtain ⟨a1, b1, c1⟩ := r1
-  obtain ⟨a2, b2, c2⟩ := r2
-  simp_all
+  grind [cases CircuitResult]
 
 lemma foldl_step_numAlloc_independent_of_constraints
-  {numAlloc : ℕ}
-  {varStore : VarStore p}
-  {constraints1 constraints2 : Prop}
-  {circuit : CircuitState p}
 :
-  (CircuitState.evalInOrder circuit σ ⟨numAlloc, varStore, constraints1⟩).numAlloc =
-  (CircuitState.evalInOrder circuit σ ⟨numAlloc, varStore, constraints2⟩).numAlloc
+  (Circuit.evalInOrder circuit σ ⟨st, varStore, constraints1⟩).st =
+  (Circuit.evalInOrder circuit σ ⟨st, varStore, constraints2⟩).st
 := by
   rcases circuit with ⟨circuit⟩
   simp only [List.size_toArray, List.foldl_toArray']
@@ -484,13 +487,9 @@ lemma foldl_step_numAlloc_independent_of_constraints
   induction circuit.reverse <;> grind
 
 lemma foldr_step_numAlloc_independent_of_constraints
-  {numAlloc : ℕ}
-  {varStore : VarStore p}
-  {constraints1 constraints2 : Prop}
-  {circuit : CircuitState p}
 :
-  (Array.foldr (λ x y => [y, σ|x]ₛ) ⟨numAlloc, varStore, constraints1⟩ circuit).numAlloc =
-  (Array.foldr (λ x y => [y, σ|x]ₛ) ⟨numAlloc, varStore, constraints2⟩ circuit).numAlloc
+  (Array.foldr (λ x y => [y, σ|x]ₛ) ⟨st, varStore, constraints1⟩ circuit).st =
+  (Array.foldr (λ x y => [y, σ|x]ₛ) ⟨st, varStore, constraints2⟩ circuit).st
 := by
   rcases circuit with ⟨circuit⟩
   rewrite [←List.reverse_reverse circuit]
@@ -499,25 +498,17 @@ lemma foldr_step_numAlloc_independent_of_constraints
   exact foldl_step_numAlloc_independent_of_constraints
 
 lemma foldr_step_numAlloc_independent_of_constraints'
-  {numAlloc : ℕ}
-  {varStore : VarStore p}
-  {constraints1 constraints2 : Prop}
-  {circuit : CircuitState p}
 :
-  (List.foldr (λ x y => [y, σ|x]ₛ) ⟨numAlloc, varStore, constraints1⟩ circuit.toList).numAlloc =
-  (List.foldr (λ x y => [y, σ|x]ₛ) ⟨numAlloc, varStore, constraints2⟩ circuit.toList).numAlloc
+  (List.foldr (λ x y => [y, σ|x]ₛ) ⟨st, varStore, constraints1⟩ circuit.toList).st =
+  (List.foldr (λ x y => [y, σ|x]ₛ) ⟨st, varStore, constraints2⟩ circuit.toList).st
 := by
   simp only [Array.foldr_toList]
   exact foldr_step_numAlloc_independent_of_constraints
 
 lemma foldl_step_varStore_independent_of_constraints
-  {numAlloc : ℕ}
-  {varStore : VarStore p}
-  {constraints1 constraints2 : Prop}
-  {circuit : CircuitState p}
 :
-  (CircuitState.evalInOrder circuit σ ⟨numAlloc, varStore, constraints1⟩).varStore =
-  (CircuitState.evalInOrder circuit σ ⟨numAlloc, varStore, constraints2⟩).varStore
+  (Circuit.evalInOrder circuit σ ⟨st, varStore, constraints1⟩).varStore =
+  (Circuit.evalInOrder circuit σ ⟨st, varStore, constraints2⟩).varStore
 := by
   rcases circuit with ⟨circuit⟩
   rewrite [←List.reverse_reverse circuit]
@@ -531,8 +522,9 @@ lemma foldl_step_varStore_independent_of_constraints
     simp at *
     rcases hd with _ | _ | _ | _
     · grind
-    · rw [Array.foldr_toList, Array.foldr_toList]
-      simp [ih]
+    · 
+      rw [Array.foldr_toList, Array.foldr_toList]
+      simp [bumpPc.eq_def, ih]
       rw [foldr_step_numAlloc_independent_of_constraints']
       congr 1
       grind
@@ -540,10 +532,10 @@ lemma foldl_step_varStore_independent_of_constraints
       simp only [step_isZero]
       unfold GetElem?.getElem?
       unfold instGetElem?ProdExprRefHashConsStZModMem
-      simp
+      simp [bumpPc.eq_def]
       rw [foldr_step_numAlloc_independent_of_constraints' (constraints2 := constraints2)]
       grind [GetElem?.getElem?, instGetElemProdExprRefHashConsStZModMem]
-    · simp
+    · simp [bumpPc.eq_def]
       rw [Array.foldr_toList, Array.foldr_toList]
       simp [foldr_step_numAlloc_independent_of_constraints' (constraints2 := constraints2)]
       simp
@@ -553,13 +545,9 @@ lemma foldl_step_varStore_independent_of_constraints
       rw [ih]
 
 lemma foldr_step_varStore_independent_of_constraints
-  {numAlloc : ℕ}
-  {varStore : VarStore p}
-  {constraints1 constraints2 : Prop}
-  {circuit : CircuitState p}
 :
-  (Array.foldr (λ x y => [y, σ|x]ₛ) ⟨numAlloc, varStore, constraints1⟩ circuit).varStore =
-  (Array.foldr (λ x y => [y, σ|x]ₛ) ⟨numAlloc, varStore, constraints2⟩ circuit).varStore
+  (Array.foldr (λ x y => [y, σ|x]ₛ) ⟨st, varStore, constraints1⟩ circuit).varStore =
+  (Array.foldr (λ x y => [y, σ|x]ₛ) ⟨st, varStore, constraints2⟩ circuit).varStore
 := by
   rcases circuit with ⟨circuit⟩
   rewrite [←List.reverse_reverse circuit]
@@ -568,28 +556,18 @@ lemma foldr_step_varStore_independent_of_constraints
   exact foldl_step_varStore_independent_of_constraints
 
 lemma foldr_step_varStore_independent_of_constraints'
-  {numAlloc : ℕ}
-  {varStore : VarStore p}
-  {constraints1 constraints2 : Prop}
-  {circuit : CircuitState p}
-  (σ : HashConsSt p)
 :
-  (List.foldr (λ x y => [y, σ|x]ₛ) ⟨numAlloc, varStore, constraints1⟩ circuit.toList).varStore =
-  (List.foldr (λ x y => [y, σ|x]ₛ) ⟨numAlloc, varStore, constraints2⟩ circuit.toList).varStore
+  (List.foldr (λ x y => [y, σ|x]ₛ) ⟨st, varStore, constraints1⟩ circuit.toList).varStore =
+  (List.foldr (λ x y => [y, σ|x]ₛ) ⟨st, varStore, constraints2⟩ circuit.toList).varStore
 := by
   simp only [Array.foldr_toList]
   exact foldr_step_varStore_independent_of_constraints
 
 @[grind .]
 lemma getElem_foldr_independent_of_constraints
-  {numAlloc : ℕ}
-  {varStore : VarStore p}
-  {constraints1 constraints2 : Prop}
-  {circuit : CircuitState p}
-  {e : ExprRef}
 :
-  (Array.foldr (λ x y => [y, σ|x]ₛ) ⟨numAlloc, varStore, constraints1⟩ circuit)[(e, σ)]? =
-  (Array.foldr (λ x y => [y, σ|x]ₛ) ⟨numAlloc, varStore, constraints2⟩ circuit)[(e, σ)]?
+  (Array.foldr (λ x y => [y, σ|x]ₛ) ⟨st, varStore, constraints1⟩ circuit)[(e!, σ)]? =
+  (Array.foldr (λ x y => [y, σ|x]ₛ) ⟨st, varStore, constraints2⟩ circuit)[(e!, σ)]?
 := by
   rcases circuit with ⟨circuit⟩
   rewrite [←List.reverse_reverse circuit]
@@ -605,9 +583,9 @@ NB this is useless now.
 -/
 -- @[grind! .] -- I don't think there's an easy way to teach grind about the `σ` under the lambda
 lemma foldr_step_varStore_independent_of_constraints''
-  {circuit : CircuitState p}
+  {circuit : Circuit p}
   {σ₁ σ₂ : CircuitResult p}
-  (h₁ : σ₁.numAlloc = σ₂.numAlloc)
+  (h₁ : σ₁.st = σ₂.st)
   (h₂ : σ₁.varStore = σ₂.varStore)
 :
   (Array.foldr (λ x y => [y, σ|x]ₛ) σ₁ circuit).varStore =
@@ -616,9 +594,9 @@ lemma foldr_step_varStore_independent_of_constraints''
   convert foldr_step_varStore_independent_of_constraints using 4 <;> grind
 
 lemma foldr_step_varStore_independent_of_constraints'''
-  {circuit : CircuitState p}
+  {circuit : Circuit p}
   {σ₁ σ₂ : CircuitResult p}
-  (h₁ : σ₁.numAlloc = σ₂.numAlloc)
+  (h₁ : σ₁.st = σ₂.st)
   (h₂ : σ₁.varStore = σ₂.varStore) :
   (List.foldr (λ x y => [y, σ|x]ₛ) σ₁ circuit.toList).varStore =
   (List.foldr (λ x y => [y, σ|x]ₛ) σ₂ circuit.toList).varStore := by
@@ -626,7 +604,7 @@ lemma foldr_step_varStore_independent_of_constraints'''
   apply foldr_step_varStore_independent_of_constraints'' <;> grind
 
 @[simp, grind .]
-lemma isSome_foldr_split {result : CircuitResult p} {circuit : CircuitState p} {e : ExprRef} :
+lemma isSome_foldr_split {result : CircuitResult p} {circuit : Circuit p} {e : ExprRef} :
   (List.foldr (fun x y => [y, σ|x]ₛ) result.split circuit.toList)[(e, σ)]?.isSome ↔
   (List.foldr (fun x y => [y, σ|x]ₛ) result circuit.toList)[(e, σ)]?.isSome := by
   rcases result
@@ -634,7 +612,7 @@ lemma isSome_foldr_split {result : CircuitResult p} {circuit : CircuitState p} {
   grind
 
 @[simp, grind .]
-lemma isSome_foldr_split' {result : CircuitResult p} {circuit : CircuitState p} {e : ExprRef} :
+lemma isSome_foldr_split' {result : CircuitResult p} {circuit : Circuit p} {e : ExprRef} :
   (Array.foldr (fun x y => [y, σ|x]ₛ) result.split circuit)[(e, σ)]?.isSome ↔
   (Array.foldr (fun x y => [y, σ|x]ₛ) result circuit)[(e, σ)]?.isSome := by
   rcases result
@@ -643,11 +621,11 @@ lemma isSome_foldr_split' {result : CircuitResult p} {circuit : CircuitState p} 
 
 lemma foldl_step_constraints_and
   {result : CircuitResult p}
-  {circuit : CircuitState p}
+  {circuit : Circuit p}
 :
-  (CircuitState.evalInOrder circuit σ result).constraints = (
+  (Circuit.evalInOrder circuit σ result).constraints = (
     result.constraints ∧
-    (CircuitState.evalInOrder circuit σ result.split).constraints
+    (Circuit.evalInOrder circuit σ result.split).constraints
   )
 := by
   rcases circuit with ⟨circuit⟩
@@ -664,12 +642,12 @@ lemma foldl_step_constraints_and
       unfold GetElem?.getElem?
       unfold instGetElem?ProdExprRefHashConsStZModMem
       rw [Array.foldr_toList, Array.foldr_toList]
-      simp [get?]
+      simp [get?, bumpPc.eq_def]
       rw [ih]
       rw [foldr_step_varStore_independent_of_constraints''' (σ₂ := result.split)] <;>
       aesop
     · rw [Array.foldr_toList, Array.foldr_toList]
-      simp [ih]
+      simp [bumpPc.eq_def, ih]
       expose_names
       rw [isSome_foldr_split]
       aesop
@@ -685,16 +663,17 @@ lemma foldl_step_constraints_and
 
 end CircuitResult
 
-namespace CircuitState
+namespace Circuit
 
-variable {p : ℕ}
+variable {p : ℕ} {circuit1 circuit2 : Circuit p} {varStore : VarStore p}
+         {st : State} {σ : HashConsSt p}
 
-def seq (circuit₁ circuit₂ : CircuitState p)
+def seq (circuit₁ circuit₂ : Circuit p)
         (varStore : VarStore p)
-        (numAlloc : ℕ)
+        (st : State)
         (σ : HashConsSt p)
 : CircuitResult p :=
-  let ⟨numAllocMid, varStoreMid, constraintsMid⟩ := eval circuit₁ varStore numAlloc σ
+  let ⟨numAllocMid, varStoreMid, constraintsMid⟩ := eval circuit₁ varStore st σ
   let ⟨numAllocPost, varStorePost, constraintsPost⟩ := eval circuit₂ varStoreMid numAllocMid σ
   ⟨numAllocPost, varStorePost, constraintsMid ∧ constraintsPost⟩
 
@@ -708,35 +687,31 @@ def unexpandSeq : Lean.PrettyPrinter.Unexpander
     `([$Γ, $numAlloc, $σ | $c₁; $c₂])
   | _ => throw ()
 
-@[simp, grind=]
-lemma numAlloc_seq {circuit1 circuit2 : CircuitState p} {varStore : VarStore p} {numAlloc : ℕ} {σ}:
-  [varStore, σ, numAlloc | circuit1; circuit2].numAlloc =
-  let mid := [varStore, σ, numAlloc|circuit1]ₑ
-  [mid.varStore, σ, mid.numAlloc|circuit2]ₑ.numAlloc
+@[simp]
+lemma numAlloc_seq :
+  [varStore, σ, st | circuit1; circuit2].st =
+  let mid := [varStore, σ, st|circuit1]ₑ
+  [mid.varStore, σ, mid.st|circuit2]ₑ.st
 := rfl
 
 @[simp]
-lemma varStore_seq (circuit1 circuit2 : CircuitState p) (varStore : VarStore p) (numAlloc : ℕ) {σ}:
-  (CircuitState.seq circuit1 circuit2 varStore numAlloc σ).varStore =
-  let mid := [varStore, σ, numAlloc|circuit1]ₑ
-  [mid.varStore, σ, mid.numAlloc|circuit2]ₑ.varStore
+lemma varStore_seq :
+  (Circuit.seq circuit1 circuit2 varStore st σ).varStore =
+  let mid := [varStore, σ, st|circuit1]ₑ
+  [mid.varStore, σ, mid.st|circuit2]ₑ.varStore
 := rfl
 
 @[simp, grind=]
-lemma constraints_seq (circuit1 circuit2 : CircuitState p) (varStore : VarStore p) (numAlloc : ℕ) {σ}:
-  (CircuitState.seq circuit1 circuit2 varStore numAlloc σ).constraints =
-  let mid := [varStore, σ, numAlloc|circuit1]ₑ
-  mid.constraints ∧ [mid.varStore, σ, mid.numAlloc|circuit2]ₑ.constraints
+lemma constraints_seq :
+  (Circuit.seq circuit1 circuit2 varStore st σ).constraints =
+  let mid := [varStore, σ, st|circuit1]ₑ
+  mid.constraints ∧ [mid.varStore, σ, mid.st|circuit2]ₑ.constraints
 := rfl
 
 @[simp, grind =]
 lemma eval_append
-  {numAlloc}
-  {circuit1 circuit2 : CircuitState p}
-  {varStore}
-  {σ}
 :
-  [varStore, σ, numAlloc | circuit1 ++ circuit2]ₑ = seq circuit1 circuit2 varStore numAlloc σ
+  [varStore, σ, st | circuit1 ++ circuit2]ₑ = seq circuit1 circuit2 varStore st σ
 := by
   simp [eval]
   ext1
@@ -748,7 +723,7 @@ lemma eval_append
 @[simp high, grind =]
 lemma eval_singleton
   {numAlloc}
-  {command : CircuitusPlanus p}
+  {command : Gate p}
   {varStore}
   {σ}
 :
@@ -759,8 +734,8 @@ lemma eval_singleton
 @[simp, grind =]
 lemma eval_cons
   {numAlloc}
-  {command : CircuitusPlanus p}
-  {circuit : CircuitState p}
+  {command : Gate p}
+  {circuit : Circuit p}
   {varStore}
   {σ}
 :
@@ -771,55 +746,55 @@ lemma eval_cons
 
 section
 
-variable {numAlloc : ℕ} {varStore : VarStore p} {e: ExprRef} {σ}
+variable {numAlloc : ℕ} {varStore : VarStore p} {e: ExprRef} {σ : HashConsSt p}
 
 @[simp, grind =]
 lemma eval_empty :
-  [varStore, σ, numAlloc | #[]]ₑ = unconstrained[numAlloc][varStore]
+  [varStore, σ, st | #[]]ₑ = unconstrained[st][varStore]
 := by rfl
 
 @[simp, grind =]
 lemma eval_empty_collection :
-  [varStore, σ, numAlloc | ∅]ₑ =
-  unconstrained[numAlloc][varStore]
+  [varStore, σ, st | ∅]ₑ =
+  unconstrained[st][varStore]
 := by rfl
 
 @[simp, grind =]
 lemma eval_eq0 :
-  [varStore, σ, numAlloc | #[.eq0 e]]ₑ =
-  unconstrained[numAlloc][varStore].step (.eq0 e) σ
+  [varStore, σ, st | #[.eq0 e]]ₑ =
+  unconstrained[st][varStore].step (.eq0 e) σ
 := by simp [eval, CircuitResult.addConstraint_unconstrained]
 
 @[simp, grind =]
 lemma eval_share :
-  [varStore, σ, numAlloc | #[.share e]]ₑ =
-  unconstrained[numAlloc][varStore].step (.share e) σ
+  [varStore, σ, st | #[.share e]]ₑ =
+  unconstrained[st][varStore].step (.share e) σ
 := by
   simp [eval]
 
 @[simp, grind =]
 lemma eval_isZero :
-  [varStore, σ, numAlloc | #[.isZero e]]ₑ =
-  unconstrained[numAlloc][varStore].step (.isZero e) σ
+  [varStore, σ, st | #[.isZero e]]ₑ =
+  unconstrained[st][varStore].step (.isZero e) σ
 := by
   simp [eval]
   rfl
 
 @[simp, grind =]
 lemma eval_num2bits {width : ℕ} :
-  [varStore, σ, numAlloc | #[.num2bits width e]]ₑ =
-  unconstrained[numAlloc][varStore].step (.num2bits width e) σ
+  [varStore, σ, st | #[.num2bits width e]]ₑ =
+  unconstrained[st][varStore].step (.num2bits width e) σ
 := by
   simp [eval]
 
 @[simp, grind =]
-lemma seq_cons_nil {cmd : CircuitusPlanus p} {circuit : CircuitState p} {varStore} {numAlloc} :
+lemma seq_cons_nil {cmd : Gate p} {circuit : Circuit p} {varStore} {numAlloc} :
   seq (⟨cmd :: circuit.toList⟩) #[] varStore numAlloc σ =
   seq #[cmd] circuit varStore numAlloc σ := by
   aesop (add simp seq)
 
 @[simp high, grind =]
-lemma seq_singleton_nil {cmd : CircuitusPlanus p} {varStore} {numAlloc} :
+lemma seq_singleton_nil {cmd : Gate p} {varStore} {numAlloc} :
   seq #[cmd] #[] varStore numAlloc σ =
   [varStore, σ, numAlloc| #[cmd]]ₑ := by
   simp [seq]
@@ -830,7 +805,7 @@ end
 -- TODO move up
 lemma step_of_refsValid_prefix
   {σ σ' : HashConsSt p}
-  {circuit : CircuitusPlanus p}
+  {circuit : Gate p}
   {result: CircuitResult p}
   (h_prefix : σ.exprs.isPrefixOf σ'.exprs)
   (h_refsValid : circuit.refsValid (σ.exprs.size))
@@ -844,7 +819,7 @@ lemma step_of_refsValid_prefix
     simp
     expose_names
     have : e < σ.exprs.size := by
-      unfold CircuitusPlanus.refsValid at h_refsValid
+      unfold Gate.refsValid at h_refsValid
       grind
     have : result[(e, σ')]? = result[(e, σ)]? := by
       unfold_projs
@@ -856,11 +831,11 @@ lemma step_of_refsValid_prefix
   }
 
 @[simp, grind _=_]
-lemma refsValid_append_iff {a b : CircuitState p} {numAlloc : ℕ}
+lemma refsValid_append_iff {a b : Circuit p} {numAlloc : ℕ}
 :
   (a ++ b).refsValid numAlloc ↔
   a.refsValid numAlloc ∧ b.refsValid numAlloc
 := by
   grind
 
-end Clap.Edsl.CircuitState
+end Clap.Edsl.Circuit
